verification/proofs/Chunk_hexVal/obl_pre_ret0_6.lean
@@ -2,4 +2,5 @@
   simp [run, step, P, hpc, hstk, State.set, pLt, pGt, *] at hrun
   subst hrun
   simp only [State.set, Nat.reduceEqDiff, reduceIte]
-  rw [hexValF_neg (by unfold digitVal; rw [if_neg (by omega), if_neg (by omega), if_neg (by omega)])]
+  rw [wrap_id' (by omega) (by omega)]
+  rw [hexValF_of (by unfold digitVal; rw [if_neg (by omega), if_pos (And.intro (by omega) (by omega))])]
