verification/proofs/Chunk_hexVal/obl_pre_ret3_7.lean
@@ -1,5 +1,0 @@
-  simp only [inv_ret0, inv_ret1, inv_ret2, inv_ret3]
-  simp [run, step, P, hpc, hstk, State.set, pLt, pGt, *] at hrun
-  subst hrun
-  simp only [State.set, Nat.reduceEqDiff, reduceIte]
-  rw [hexValF_neg (by unfold digitVal; rw [if_neg (by omega), if_neg (by omega), if_neg (by omega)])]
